P1-PL/Interpreter.v
@@ -4,11 +4,10 @@ From Coq Require Import List.
 Import ListNotations.
 From FirstProject Require Import Imp Maps.
 
-
 Inductive interpreter_result : Type :=
-  | Success (s: state * (list (state*com)))
-  | Fail
-  | OutOfGas.
+  | Success (s: state * (list (state*com))) (i: nat)
+  | Fail (er: string) (i: nat) 
+  | OutOfGas (er: string).
 
 (** We can improve the readability of this version by introducing a
     bit of auxiliary notation to hide the plumbing involved in
@@ -16,10 +15,14 @@ Inductive interpreter_result : Type :=
 
 Notation "'CHECKSUC' x y <== e1 'IN' e2"
    := (match e1 with
-       | Success (x, y) => e2
+       | Success (x, y) (i) => e2
        | a => a
        end)
    (at level 10, x at next level, y at next level, e1 at next level, e2 at next level).
+
+(* Error messages for outOfGas and Fail *)
+Definition outOfGasError : string := "Ran out of Gas".
+Definition failError : string := "No continuation found in conditional guard".
 
 (**
   2.1. Implement ceval_step as specified. To improve readability,
@@ -29,13 +32,13 @@ Notation "'CHECKSUC' x y <== e1 'IN' e2"
 Fixpoint ceval_step (st : state) (c : com) (continuation: list (state * com)) (i : nat)
                     : interpreter_result :=
   match i with
-  | O => OutOfGas
+  | O => OutOfGas outOfGasError
   | S i' => 
       match c with
       | <{ skip }> =>
-          Success (st, continuation)
+          Success (st, continuation) i
       | <{ l := a1 }> =>
-          Success ((l !-> aeval st a1 ; st), continuation)
+          Success ((l !-> aeval st a1 ; st), continuation) i
       | <{ c1 ; c2 }> =>
           CHECKSUC st' cont' <== (ceval_step st c1 continuation i') IN
               (ceval_step st' c2 cont' i')
@@ -49,76 +52,79 @@ Fixpoint ceval_step (st : state) (c : com) (continuation: list (state * com)) (i
             CHECKSUC st' cont' <== (ceval_step st c1 continuation i') IN
               (ceval_step st' c cont' i')
           else 
-            Success (st, continuation)
+            Success (st, continuation) i
       | <{ x1 !! x2 }> =>
           ceval_step st x1 ((st, x2) :: continuation) i'
       | <{ x -> y }> => 
-          if (beval st b) then
-            ceval_step st c (tail continuation) i'
+          if (beval st x) then
+            ceval_step st y continuation i'
           else 
             match continuation with
-              | [] => Fail
-              | ((st', x2') :: t) => match i' with
-                | 0 => OutOfGas
+              | [] => Fail failError i
+              | ((st', x2') :: t) => 
+                match i' with
+                | 0 => OutOfGas outOfGasError
                 | S i'' => CHECKSUC st'' cont' <== (ceval_step st' x2' t i'') IN
-              (ceval_step st'' c cont' i'')
+                           (ceval_step st'' c cont' i'')
+                end
             end
       end
   end.
 
 (* Helper functions that help with running the interpreter *)
 Inductive show_result : Type :=
-  | OK (st: list (string*nat))
-  | KO
-  | OOG.
+  | OK (st: list (string*nat)) (i: nat)
+  | KO (er: string) (i: nat)
+  | OOG (er: string).
 
 Open Scope string_scope.
 Definition run_interpreter (st: state) (c:com) (n:nat) :=
   match (ceval_step st c [] n) with
-    | OutOfGas => OOG
-    | Fail => KO
-    | Success (st', _) => OK [("X", st' X); ("Y", st' Y); ("Z", st' Z)]
+    | OutOfGas a => OOG a
+    | Fail a i => KO a i
+    | Success (st', _) (i) => OK [("X", st' X); ("Y", st' Y); ("Z", st' Z)] i
   end.
 
 (* Tests are provided to ensure that your interpreter is working for these examples *)
 Example test_1: 
-  run_interpreter (X !-> 5) <{skip}> 1 = OK [("X", 5); ("Y", 0); ("Z", 0)].
+  run_interpreter (X !-> 5) <{skip}> 1 = OK [("X", 5); ("Y", 0); ("Z", 0)] 1.
 Proof. auto. Qed.
 
 Example test_2: 
-  run_interpreter (X !-> 5) <{ X:= X+1 }> 1 = OK [("X", 6); ("Y", 0); ("Z", 0)].
+  run_interpreter (X !-> 5) <{ X:= X+1 }> 1 = OK [("X", 6); ("Y", 0); ("Z", 0)] 1.
 Proof. auto. Qed.
 
 Example test_3: 
-  run_interpreter (X !-> 5) <{ X:= X+1; X:=X+2; Y:=Y+1 }> 3 = OK [("X", 8); ("Y", 1); ("Z", 0)].
+  run_interpreter (X !-> 5) <{ X:= X+1; X:=X+2; Y:=Y+1 }> 3 = OK [("X", 8); ("Y", 1); ("Z", 0)] 1.
 Proof. auto. Qed.
 
+
 Example test_4: 
-  run_interpreter (X !-> 5) <{ X:= X+1; X:=X+2; Y:=Y+1 }> 2 = OOG.
+  run_interpreter (X !-> 5) <{ X:= X+1; X:=X+2; Y:=Y+1 }> 2 = OOG outOfGasError.
 Proof. auto. Qed.
 
 Example test_5:
-  run_interpreter (X !-> 5) <{ X:= X+1; X=5 -> skip }> 2 = KO.
+  run_interpreter (X !-> 5) <{ X:= X+1; X=5 -> skip }> 2 = KO failError 1.
 Proof. auto. Qed.
 
 Example test_6:
-  run_interpreter (X !-> 5) <{ X:= X+1; X=5 -> skip }> 1 = OOG.
+  run_interpreter (X !-> 5) <{ X:= X+1; X=5 -> skip }> 1 = OOG outOfGasError.
 Proof. auto. Qed.
 
 Example test_7:
-  run_interpreter (X !-> 5) <{ X:= X+1; X=6 -> skip }> 3 = OK [("X", 6); ("Y", 0); ("Z", 0)].
+  run_interpreter (X !-> 5) <{ X:= X+1; X=6 -> skip }> 3 = OK [("X", 6); ("Y", 0); ("Z", 0)] 1.
 Proof. auto. Qed.
 
 Example test_8:
-  run_interpreter (X !-> 5) <{ (X := 1 !! X := 2); (X = 2) -> X:=3 }> 4 = OOG.
+  run_interpreter (X !-> 5) <{ (X := 1 !! X := 2); (X = 2) -> X:=3 }> 4 = OOG outOfGasError.
 Proof. auto. Qed.
 
 Example test_9:
-  run_interpreter (X !-> 5) <{ (X := 1 !! X := 2); (X = 2) -> X:=3 }> 5 = OK [("X", 3); ("Y", 0); ("Z", 0)].
+  run_interpreter (X !-> 5) <{ (X := 1 !! X := 2); (X = 2) -> X:=3 }> 5 = OK [("X", 3); ("Y", 0); ("Z", 0)] 1.
 Proof. auto. Qed.
 
 Example test_10:
-  run_interpreter (X !-> 5) <{ (X:=1 !! (X:=2; Y:=1));X=2 -> skip }> 5 = OK [("X", 2); ("Y", 1); ("Z", 0)].
+  run_interpreter (X !-> 5) <{ (X:=1 !! (X:=2; Y:=1));X=2 -> skip }> 5 = OK [("X", 2); ("Y", 1); ("Z", 0)] 1.
 Proof. auto. Qed.
 
 Example test_11:
@@ -129,15 +135,16 @@ Example test_11:
       Y=5 -> skip
   }>
   8 
-  = OK [("X", 0); ("Y", 5); ("Z", 0)].
+  = OK [("X", 0); ("Y", 5); ("Z", 0)] 6. 
 Proof. auto. Qed.
 
 
 
 (**
   2.2: Prove p1_equals_p2. Recall that p1 and p2 are defined in Imp.v
+**)
 
-
+(*
 Theorem p1_equals_p2: forall st cont,
   (exists i0,
     (forall i1, i1 >= i0 -> ceval_step st p1 cont i1 = ceval_step st p2 cont i1)).
@@ -153,7 +160,6 @@ Proof.
     ------- intros. simpl. reflexivity.
     ------- intros. simpl. reflexivity.
 Qed.
-
 *)
 
 
